theories/ordinals/Ackermann/PA.v
@@ -53,7 +53,7 @@ Definition open :=
   Formula_rec LNT (fun _ => Formula) (fun t t0 : Term => equal t t0)
     (fun (r : Relations LNT) 
          (ts : Terms (arity LNT (inl (Functions LNT) r))) =>
-       atomic LNT r ts) 
+       atomic r ts) 
     (fun (f : Formula) _ (f0 : Formula) _ => impH f f0)
     (fun (f : Formula) _ => notH f)
     (fun (n : nat) _ (recf : Formula) => recf).
